Switch to a shallower embedding

src/MicroSail/Syntax.v
@@ -40,519 +40,113 @@ From MicroSail Require Export
 
 Set Implicit Arguments.
 
-Module Type TypeKit.
+Local Definition Cont (R A : Type) : Type := (A -> R) -> R.
 
-  (* Names of enum type constructors. *)
-  Parameter Inline 𝑬 : Set. (* input: \MIE *)
-  (* Names of union type constructors. *)
-  Parameter Inline 𝑻   : Set. (* input: \MIT *)
-  (* Names of record type constructors. *)
-  Parameter Inline 𝑹  : Set. (* input: \MIR *)
-  (* Names of expression variables. *)
-  Parameter Inline 𝑿 : Set. (* input: \MIX *)
-  (* For name resolution we rely on decidable equality of expression
-     variables. The functions in this module resolve to the closest binding
-     of an equal name and fill in the de Bruijn index automatically from
-     a successful resolution.
-  *)
-  Parameter Inline 𝑿_eq_dec : forall x y : 𝑿, {x=y}+{~x=y}.
+Class Blastable (A : Set) : Type :=
+  { blast : A -> Cont Prop A;
+    blast_sound:
+      forall (a : A) (k : A -> Prop),
+        blast a k <-> k a
+  } .
 
-End TypeKit.
+Program Instance blastable_bool : Blastable bool :=
+  {| blast := fun b k => (b = true -> k true) /\ (b = false -> k false) |}.
+Solve All Obligations with destruct a; intuition.
 
-Module Types (Export typekit : TypeKit).
+Program Instance blastable_int : Blastable Z :=
+  { blast := fun z k => k z }.
+Solve All Obligations with intuition.
 
-  Inductive Ty : Set :=
-  | ty_int
-  | ty_bool
-  | ty_bit
-  | ty_string
-  | ty_list (σ : Ty)
-  | ty_prod (σ τ : Ty)
-  | ty_sum  (σ τ : Ty)
-  | ty_unit
-  | ty_enum (E : 𝑬)
-  (* Experimental features. These are still in flux. *)
-  | ty_tuple (σs : Ctx Ty)
-  | ty_union (T : 𝑻)
-  | ty_record (R : 𝑹)
-  .
+Program Instance blastable_prod {A B : Set} : Blastable (A * B) :=
+  { blast := fun ab k => k (fst ab , snd ab) }.
+Solve All Obligations with intuition.
 
-End Types.
+Program Instance blastable_sum {A B : Set} : Blastable (A + B) :=
+  { blast := fun ab k =>
+               (forall (a : A), ab = inl a -> k (inl a)) /\
+               (forall (b : B), ab = inr b -> k (inr b)) }.
+Solve All Obligations with destruct a; intuition; congruence.
 
 (******************************************************************************)
 
-Module Type TermKit (typekit : TypeKit).
-  Module TY := Types typekit.
-  Export TY.
-
-  (* Names of enum data constructors. *)
-  Parameter Inline 𝑬𝑲 : 𝑬 -> Set.
-  (* Names of union data constructors. *)
-  Parameter Inline 𝑲  : 𝑻 -> Set.
-  (* Union data constructor field type *)
-  Parameter Inline 𝑲_Ty : forall (T : 𝑻), 𝑲 T -> Ty.
-  (* Record field names. *)
-  Parameter Inline 𝑹𝑭  : Set.
-  (* Record field types. *)
-  Parameter Inline 𝑹𝑭_Ty : 𝑹 -> Ctx (𝑹𝑭 * Ty).
+Module Type TermKit.
 
   (* Names of functions. *)
-  Parameter Inline 𝑭  : Ctx (𝑿 * Ty) -> Ty -> Set.
+  Parameter Inline 𝑭  : Ctx Set -> Set -> Set.
 
 End TermKit.
 
-Module Terms (typekit : TypeKit) (termkit : TermKit typekit).
+Module Terms (termkit : TermKit).
   Export termkit.
 
-  Section Literals.
-
-    Inductive Bit : Set := bitzero | bitone.
-
-    (* Ideally we want object language literals to coincide with meta-language
-       values to get sexy looking predicates. See the definition of Lit below.
-       Unfortunately our setup of union and record types essentially is a giant
-       mutually recursive family of types and hence Lit below would not
-       terminate if it were directly extended to unions/records. TaggedLit is an
-       inductive and therefore terminating definition of the recursive family of
-       types and our current solution to the problem.
-
-       Because Sail does not allow recursive types the records and unions in the
-       generated output will form a strict DAG. Enforcing a topological sorting
-       is more work than simply allowing recursive definitions. Another option
-       is to encode the DAG as a well-founded relation between type constructor
-       names an defining Lit by well-founded recursion. This would need some
-       investigation.
-
-       The ideal way to add recursive types would be to only introduce tags at
-       recursive positions. For instance writing Lit as a recursive definition
-       of a functor and using that in the definition of tagged:
-
-         Fixpoint Lit (tl : Ty -> Set) (σ : Ty) {struct σ} : Set := match σ with
-           ... end.
-
-         Inductive TaggedLit (σ : Ty) : Set := | tagged : Lit TaggedLit σ ->
-         TaggedLit σ.
-
-       But currently Coq's strict-positivity checker is not smart enough to deem
-       it safe. (Agda excepts this definition). So TaggedLit adds tags
-       everywhere.
-     *)
-    Inductive TaggedLit : Ty -> Set :=
-    | taglit_int           : Z -> TaggedLit (ty_int)
-    | taglit_bool          : bool -> TaggedLit (ty_bool)
-    | taglit_bit           : Bit -> TaggedLit (ty_bit)
-    | taglit_string        : string -> TaggedLit (ty_string)
-    | taglit_list   σ'     : list (TaggedLit σ') -> TaggedLit (ty_list σ')
-    | taglit_prod   σ1 σ2  : TaggedLit σ1 * TaggedLit σ2 -> TaggedLit (ty_prod σ1 σ2)
-    | taglit_sum    σ1 σ2  : TaggedLit σ1 + TaggedLit σ2 -> TaggedLit (ty_sum σ1 σ2)
-    | taglit_unit          : TaggedLit (ty_unit)
-    | taglit_enum (E : 𝑬) (K : 𝑬𝑲 E) : TaggedLit (ty_enum E)
-    (* Experimental features *)
-    | taglit_tuple σs      : Env TaggedLit σs -> TaggedLit (ty_tuple σs)
-    | taglit_union (T : 𝑻) (K : 𝑲 T) : TaggedLit (𝑲_Ty K) -> TaggedLit (ty_union T)
-    | taglit_record (R : 𝑹) : Env' TaggedLit (𝑹𝑭_Ty R) -> TaggedLit (ty_record R).
-
-    Global Arguments taglit_enum : clear implicits.
-    Global Arguments taglit_tuple {_} _.
-    Global Arguments taglit_union {_} _ _.
-    Global Arguments taglit_record : clear implicits.
-
-    Fixpoint Lit (σ : Ty) : Set :=
-      match σ with
-      | ty_int => Z
-      | ty_bool => bool
-      | ty_bit => Bit
-      | ty_string => string
-      | ty_list σ' => list (Lit σ')
-      | ty_prod σ1 σ2 => Lit σ1 * Lit σ2
-      | ty_sum σ1 σ2 => Lit σ1 + Lit σ2
-      | ty_unit => unit
-      | ty_enum E => 𝑬𝑲 E
-      (* Experimental features *)
-      | ty_tuple σs => Env TaggedLit σs
-      | ty_union T => { K : 𝑲 T & TaggedLit (𝑲_Ty K) }
-      | ty_record R => Env' TaggedLit (𝑹𝑭_Ty R)
-      end%type.
-
-    Fixpoint untag {σ : Ty} (v : TaggedLit σ) : Lit σ :=
-      match v with
-      | taglit_int z        => z
-      | taglit_bool b       => b
-      | taglit_bit b        => b
-      | taglit_string s     => s
-      | taglit_list ls      => List.map untag ls
-      | taglit_prod (l , r) => (untag l , untag r)
-      | taglit_sum (inl v)  => inl (untag v)
-      | taglit_sum (inr v)  => inr (untag v)
-      | taglit_unit         => tt
-      | taglit_enum E K     => K
-      (* Experimental features *)
-      | taglit_tuple ls     => ls
-      | taglit_union K l    => existT _ K l
-      | taglit_record R t   => t
-      end.
-
-    Fixpoint tag (σ : Ty) {struct σ} : Lit σ -> TaggedLit σ :=
-      match σ with
-      | ty_int => fun (l : Lit ty_int) => taglit_int l
-      | ty_bool => taglit_bool
-      | ty_bit => taglit_bit
-      | ty_string => taglit_string
-      | ty_list σ =>
-        fun l => taglit_list (List.map (tag σ) l)
-      | ty_prod σ1 σ2 =>
-        fun l => let (l1, l2) := l in
-                 taglit_prod (tag σ1 l1, tag σ2 l2)
-      | ty_sum σ1 σ2 =>
-        fun l : Lit (ty_sum σ1 σ2) =>
-          match l with
-          | inl l => taglit_sum (inl (tag σ1 l))
-          | inr l => taglit_sum (inr (tag σ2 l))
-          end
-      | ty_unit => fun _ => taglit_unit
-      | ty_enum E => taglit_enum E
-      | ty_tuple σs => taglit_tuple
-      | ty_union T => fun Ktl => let (K, tl) := Ktl in taglit_union K tl
-      | ty_record R => taglit_record R
-      end.
-
-  End Literals.
-
-  Section Expressions.
-
-    (* Intrinsically well-typed expressions. The context Γ of mutable variables
-       contains names 𝑿 and types Ty, but the names are not computationally
-       relevant. The underlying representation is still a de Bruijn index based
-       one. The names are meant for human consumption and we also provide name
-       resolution infrastructure in the NameResolution module to fill in de
-       Bruijn indices automatically.
-
-       The de Bruijn indices are wrapped together with a resolution proof in the
-       InCtx type class, which currently does not have any global instances. We
-       do have local implicit instances like for example in the exp_var
-       constructor below and use the type class mechanism to copy these
-       locally. *)
-    Inductive Exp (Γ : Ctx (𝑿 * Ty)) : Ty -> Set :=
-    | exp_var     (x : 𝑿) (σ : Ty) {xInΓ : InCtx (x , σ) Γ} : Exp Γ σ
-    | exp_lit     (σ : Ty) : Lit σ -> Exp Γ σ
-    | exp_plus    (e1 e2 : Exp Γ ty_int) : Exp Γ ty_int
-    | exp_times   (e1 e2 : Exp Γ ty_int) : Exp Γ ty_int
-    | exp_minus   (e1 e2 : Exp Γ ty_int) : Exp Γ ty_int
-    | exp_neg     (e : Exp Γ ty_int) : Exp Γ ty_int
-    | exp_eq      (e1 e2 : Exp Γ ty_int) : Exp Γ ty_bool
-    | exp_le      (e1 e2 : Exp Γ ty_int) : Exp Γ ty_bool
-    | exp_lt      (e1 e2 : Exp Γ ty_int) : Exp Γ ty_bool
-    | exp_gt      (e1 e2 : Exp Γ ty_int) : Exp Γ ty_bool
-    | exp_and     (e1 e2 : Exp Γ ty_bool) : Exp Γ ty_bool
-    | exp_not     (e : Exp Γ ty_bool) : Exp Γ ty_bool
-    | exp_pair    {σ1 σ2 : Ty} (e1 : Exp Γ σ1) (e2 : Exp Γ σ2) : Exp Γ (ty_prod σ1 σ2)
-    | exp_inl     {σ1 σ2 : Ty} : Exp Γ σ1 -> Exp Γ (ty_sum σ1 σ2)
-    | exp_inr     {σ1 σ2 : Ty} : Exp Γ σ2 -> Exp Γ (ty_sum σ1 σ2)
-    | exp_list    {σ : Ty} (es : list (Exp Γ σ)) : Exp Γ (ty_list σ)
-    | exp_cons    {σ : Ty} (h : Exp Γ σ) (t : Exp Γ (ty_list σ)) : Exp Γ (ty_list σ)
-    | exp_nil     {σ : Ty} : Exp Γ (ty_list σ)
-    (* Experimental features *)
-    | exp_tuple   {σs : Ctx Ty} (es : Env (Exp Γ) σs) : Exp Γ (ty_tuple σs)
-    | exp_projtup {σs : Ctx Ty} (e : Exp Γ (ty_tuple σs)) (n : nat) {σ : Ty}
-                  {p : ctx_nth_is σs n σ} : Exp Γ σ
-    | exp_union   {T : 𝑻} (K : 𝑲 T) (e : Exp Γ (𝑲_Ty K)) : Exp Γ (ty_union T)
-    | exp_record  (R : 𝑹) (es : Env' (Exp Γ) (𝑹𝑭_Ty R)) : Exp Γ (ty_record R)
-    | exp_projrec {R : 𝑹} (e : Exp Γ (ty_record R)) (rf : 𝑹𝑭) {σ : Ty}
-                  {rfInR : InCtx (rf , σ) (𝑹𝑭_Ty R)} : Exp Γ σ
-    | exp_builtin {σ τ : Ty} (f : Lit σ -> Lit τ) (e : Exp Γ σ) : Exp Γ τ.
-    Bind Scope exp_scope with Exp.
-
-    Global Arguments exp_var {_} _ {_ _}.
-    Global Arguments exp_tuple {_ _} _%exp.
-    Global Arguments exp_union {_} _ _.
-    Global Arguments exp_record {_} _ _.
-    Global Arguments exp_projrec {_ _} _ _ {_ _}.
-
-    Import EnvNotations.
-
-    Definition LocalStore (Γ : Ctx (𝑿 * Ty)) : Set := Env' Lit Γ.
-
-    Fixpoint evalTagged {Γ : Ctx (𝑿 * Ty)} {σ : Ty} (e : Exp Γ σ) (δ : LocalStore Γ) {struct e} : TaggedLit σ :=
-      match e in (Exp _ t) return (TaggedLit t) with
-      | exp_var x => tag _ (δ ! x)
-      | exp_lit _ σ0 l => tag σ0 l
-      | exp_plus e1 e2 => taglit_int (untag (evalTagged e1 δ) + untag (evalTagged e2 δ))
-      | exp_times e1 e2 => taglit_int (untag (evalTagged e1 δ) * untag (evalTagged e2 δ))
-      | exp_minus e1 e2 => taglit_int (untag (evalTagged e1 δ) - untag (evalTagged e2 δ))
-      | exp_neg e0 => taglit_int (- untag (evalTagged e0 δ))
-      | exp_eq e1 e2 => taglit_bool (untag (evalTagged e1 δ) =? untag (evalTagged e2 δ))%Z
-      | exp_le e1 e2 => taglit_bool (untag (evalTagged e1 δ) <=? untag (evalTagged e2 δ))%Z
-      | exp_lt e1 e2 => taglit_bool (untag (evalTagged e1 δ) <? untag (evalTagged e2 δ))%Z
-      | exp_gt e1 e2 => taglit_bool (untag (evalTagged e1 δ) >? untag (evalTagged e2 δ))%Z
-      | exp_and e1 e2 => taglit_bool (untag (evalTagged e1 δ) && untag (evalTagged e2 δ))
-      | exp_not e0 => taglit_bool (negb (untag (evalTagged e0 δ)))
-      | @exp_pair _ σ1 σ2 e1 e2 => taglit_prod (evalTagged e1 δ, evalTagged e2 δ)
-      | @exp_inl _ σ1 σ2 e0 => taglit_sum (inl (evalTagged e0 δ))
-      | @exp_inr _ σ1 σ2 e0 => taglit_sum (inr (evalTagged e0 δ))
-      | @exp_list _ σ0 es => taglit_list (List.map (fun e0 : Exp Γ σ0 => evalTagged e0 δ) es)
-      | @exp_cons _ σ0 e1 e2 =>
-        (* This is less efficient than it could be. It's untagging the head and
-           the whole list while it would only need to destruct (evalTagged e2
-           δ). *)
-        tag (ty_list σ0) (cons (untag (evalTagged e1 δ)) (untag (evalTagged e2 δ)))
-      | @exp_nil _ σ0 => taglit_list nil
-      | @exp_tuple _ σs es =>
-        let evalsTagged := fix evalsTagged {σs : Ctx Ty} (es : Env (Exp Γ) σs) : Env TaggedLit σs :=
-                             match es with
-                             | env_nil => env_nil
-                             | env_snoc es σ e => env_snoc (evalsTagged es) σ (evalTagged e δ)
-                             end
-        in taglit_tuple (evalsTagged es)
-      | @exp_projtup _ σs e0 n σ0 p => env_lookup (untag (evalTagged e0 δ)) (Build_InCtx _ _ n p)
-      | @exp_union _ T K e0 => taglit_union K (evalTagged e0 δ)
-      | exp_record R es =>
-        let evalsTagged := fix evalsTagged {rfs : Ctx (𝑹𝑭 * Ty)} (es : Env' (Exp Γ) rfs) : Env' TaggedLit rfs :=
-                             match es with
-                             | env_nil => env_nil
-                             | env_snoc es σ e => env_snoc (evalsTagged es) σ (evalTagged e δ)
-                             end
-        in taglit_record R (evalsTagged es)
-      | @exp_projrec _ R e0 rf σ0 rfInR => env_lookup (untag (evalTagged e0 δ)) rfInR
-      | @exp_builtin _ σ0 τ f e0 => tag τ (f (untag (evalTagged e0 δ)))
-      end.
-
-    Fixpoint eval {Γ : Ctx (𝑿 * Ty)} {σ : Ty} (e : Exp Γ σ) (δ : LocalStore Γ) {struct e} : Lit σ :=
-      match e in (Exp _ t) return (Lit t) with
-      | exp_var x           => δ ! x
-      | exp_lit _ _ l       => l
-      | exp_plus e1 e2      => Z.add (eval e1 δ) (eval e2 δ)
-      | exp_times e1 e2     => Z.mul (eval e1 δ) (eval e2 δ)
-      | exp_minus e1 e2     => Z.sub (eval e1 δ) (eval e2 δ)
-      | exp_neg e           => Z.opp (eval e δ)
-      | exp_eq e1 e2        => Z.eqb (eval e1 δ) (eval e2 δ)
-      | exp_le e1 e2        => Z.leb (eval e1 δ) (eval e2 δ)
-      | exp_lt e1 e2        => Z.ltb (eval e1 δ) (eval e2 δ)
-      | exp_gt e1 e2        => Z.gtb (eval e1 δ) (eval e2 δ)
-      | exp_and e1 e2       => andb (eval e1 δ) (eval e2 δ)
-      | exp_not e           => negb (eval e δ)
-      | exp_pair e1 e2      => pair (eval e1 δ) (eval e2 δ)
-      | exp_inl e           => inl (eval e δ)
-      | exp_inr e           => inr (eval e δ)
-      | exp_list es         => List.map (fun e => eval e δ) es
-      | exp_cons e1 e2      => cons (eval e1 δ) (eval e2 δ)
-      | exp_nil _           => nil
-      | exp_tuple es        => env_map (fun τ e => evalTagged e δ) es
-      | @exp_projtup _ σs e n σ p => untag (env_lookup (eval e δ) (Build_InCtx _ _ n p))
-      | exp_union T K e     => existT _ K (evalTagged e δ)
-      | exp_record R es     => env_map (fun τ e => evalTagged e δ) es
-      | exp_projrec e rf    => untag (eval e δ ! rf)
-      | exp_builtin f e     => f (eval e δ)
-      end.
-
-    Definition evals {Γ Δ} (es : Env' (Exp Γ) Δ) (δ : LocalStore Γ) : LocalStore Δ :=
-      env_map (fun xτ e => eval e δ) es.
-
-  End Expressions.
-  Bind Scope exp_scope with Exp.
+  Definition Lit (A : Set) : Set := A.
+  Arguments Lit / _.
+  Definition LocalStore (Γ : Ctx Set) : Type := Env Lit Γ.
 
   Section Statements.
 
-    Inductive TuplePat : Ctx Ty -> Ctx (𝑿 * Ty) -> Set :=
-    | tuplepat_nil  : TuplePat ctx_nil ctx_nil
-    | tuplepat_snoc
-        {σs : Ctx Ty} {Δ : Ctx (𝑿 * Ty)}
-        (pat : TuplePat σs Δ) {σ : Ty} (x : 𝑿) :
-        TuplePat (ctx_snoc σs σ) (ctx_snoc Δ (x , σ)).
-    Bind Scope pat_scope with TuplePat.
+    Inductive Stm : Set -> Type :=
+    | stm_lit        {σ : Set} (v : σ) : Stm σ
+    | stm_app        {Δ σ} (f : 𝑭 Δ σ) (es : Env Lit Δ) : Stm σ
+    | stm_if         {τ : Set} (b : bool) (s1 s2 : Stm τ) : Stm τ
+    | stm_assert     (b : bool) (e2 : string) : Stm bool
+    | stm_exit       (τ : Set) (s : string) : Stm τ
+    (* | stm_match      {σ τ : Set} {σMatch : Blastable σ} (s : Stm σ) (k : σ -> Stm τ) : Stm τ *)
+    | stm_bind       {σ τ : Set} {σMatch : Blastable σ} (s : Stm σ) (k : σ -> Stm τ) : Stm τ.
 
-    Inductive RecordPat : Ctx (𝑹𝑭 * Ty) -> Ctx (𝑿 * Ty) -> Set :=
-    | recordpat_nil  : RecordPat ctx_nil ctx_nil
-    | recordpat_snoc
-        {rfs : Ctx (𝑹𝑭 * Ty)} {Δ : Ctx (𝑿 * Ty)}
-        (pat : RecordPat rfs Δ) (rf : 𝑹𝑭) {τ : Ty} (x : 𝑿) :
-        RecordPat (ctx_snoc rfs (rf , τ)) (ctx_snoc Δ (x , τ)).
-    Bind Scope pat_scope with RecordPat.
-
-    Inductive Stm (Γ : Ctx (𝑿 * Ty)) : Ty -> Set :=
-    | stm_lit        {τ : Ty} (l : Lit τ) : Stm Γ τ
-    | stm_exp        {τ : Ty} (e : Exp Γ τ) : Stm Γ τ
-    | stm_let        (x : 𝑿) (τ : Ty) (s : Stm Γ τ) {σ : Ty} (k : Stm (ctx_snoc Γ (x , τ)) σ) : Stm Γ σ
-    | stm_let'       (Δ : Ctx (𝑿 * Ty)) (δ : LocalStore Δ) {σ : Ty} (k : Stm (ctx_cat Γ Δ) σ) : Stm Γ σ
-    | stm_assign     (x : 𝑿) (τ : Ty) {xInΓ : InCtx (x , τ) Γ} (e : Exp Γ τ) : Stm Γ τ
-    | stm_app        {Δ σ} (f : 𝑭 Δ σ) (es : Env' (Exp Γ) Δ) : Stm Γ σ
-    | stm_app'       (Δ : Ctx (𝑿 * Ty)) (δ : LocalStore Δ) (τ : Ty) (s : Stm Δ τ) : Stm Γ τ
-    | stm_if         {τ : Ty} (e : Exp Γ ty_bool) (s1 s2 : Stm Γ τ) : Stm Γ τ
-    | stm_seq        {τ : Ty} (e : Stm Γ τ) {σ : Ty} (k : Stm Γ σ) : Stm Γ σ
-    | stm_assert     (e1 : Exp Γ ty_bool) (e2 : Exp Γ ty_string) : Stm Γ ty_bool
-    (* | stm_while      (w : 𝑾 Γ) (e : Exp Γ ty_bool) {σ : Ty} (s : Stm Γ σ) -> Stm Γ ty_unit *)
-    | stm_exit       (τ : Ty) (s : Lit ty_string) : Stm Γ τ
-    | stm_match_list {σ τ : Ty} (e : Exp Γ (ty_list σ)) (alt_nil : Stm Γ τ)
-      (xh xt : 𝑿) (alt_cons : Stm (ctx_snoc (ctx_snoc Γ (xh , σ)) (xt , ty_list σ)) τ) : Stm Γ τ
-    | stm_match_sum  {σinl σinr τ : Ty} (e : Exp Γ (ty_sum σinl σinr))
-      (xinl : 𝑿) (alt_inl : Stm (ctx_snoc Γ (xinl , σinl)) τ)
-      (xinr : 𝑿) (alt_inr : Stm (ctx_snoc Γ (xinr , σinr)) τ) : Stm Γ τ
-    | stm_match_pair {σ1 σ2 τ : Ty} (e : Exp Γ (ty_prod σ1 σ2))
-      (xl xr : 𝑿) (rhs : Stm (ctx_snoc (ctx_snoc Γ (xl , σ1)) (xr , σ2)) τ) : Stm Γ τ
-    | stm_match_enum {E : 𝑬} (e : Exp Γ (ty_enum E)) {τ : Ty}
-      (alts : forall (K : 𝑬𝑲 E), Stm Γ τ) : Stm Γ τ
-    | stm_match_tuple {σs : Ctx Ty} {Δ : Ctx (𝑿 * Ty)} (e : Exp Γ (ty_tuple σs))
-      (p : TuplePat σs Δ) {τ : Ty} (rhs : Stm (ctx_cat Γ Δ) τ) : Stm Γ τ
-    | stm_match_union {T : 𝑻} (e : Exp Γ (ty_union T)) {τ : Ty}
-      (* An earlier definition of stm_match_union used a "list of pairs"
-          (alts : forall (K : 𝑲 T), { x : 𝑿 & Stm (ctx_snoc Γ (x , 𝑲_Ty K)) τ})
-         to define alternatives, which packs the variable name x for the field
-         of the union neatly together with the right hand side. Unfortunately,
-         due toe the sigma type constructor the derived induction principle is
-         not strong enough. It's possible to write a better induction principle
-         by hand, but since the AST is still in flux this is too much of a
-         burden to keep updated. Instead we use two "lists", one for the
-         variable names and one for the RHSs, which separates them lexically,
-         but gives a better induction principle. *)
-      (altx : forall (K : 𝑲 T), 𝑿)
-      (alts : forall (K : 𝑲 T), Stm (ctx_snoc Γ (altx K , 𝑲_Ty K)) τ) : Stm Γ τ
-    | stm_match_record {R : 𝑹} {Δ : Ctx (𝑿 * Ty)} (e : Exp Γ (ty_record R))
-      (p : RecordPat (𝑹𝑭_Ty R) Δ) {τ : Ty} (rhs : Stm (ctx_cat Γ Δ) τ) : Stm Γ τ
-    | stm_bind   {σ τ : Ty} (s : Stm Γ σ) (k : Lit σ -> Stm Γ τ) : Stm Γ τ.
-
-    Global Arguments stm_lit {_} _ _.
-    Global Arguments stm_exp {_ _} _.
-    Global Arguments stm_let {_} _ _ _ {_} _.
-    Global Arguments stm_let' {_ _} _ {_} _.
-    Global Arguments stm_assign {_} _ {_ _} _.
-    Global Arguments stm_app {_%ctx _%ctx _} _ _%exp.
-    Global Arguments stm_app' {_} _ _ _ _.
-    Global Arguments stm_if {_ _} _ _ _.
-    Global Arguments stm_seq {_ _} _ {_} _.
-    Global Arguments stm_assert {_} _ _.
-    Global Arguments stm_exit {_} _ _.
-    Global Arguments stm_match_list {_ _ _} _ _ _ _ _.
-    Global Arguments stm_match_sum {_ _ _ _} _ _ _ _ _.
-    Global Arguments stm_match_pair {_ _ _ _} _ _ _ _.
-    Global Arguments stm_match_enum {_} _ _ {_} _.
-    Global Arguments stm_match_tuple {_ _ _} _ _%pat {_} _.
-    Global Arguments stm_match_union {_} _ _ {_} _ _.
-    Global Arguments stm_match_record {_} _ {_} _ _ {_} _.
+    Global Arguments stm_lit _.
+    Global Arguments stm_app {_%ctx _} _ _%exp.
+    Global Arguments stm_if {_} _ _ _.
+    Global Arguments stm_assert _ _.
+    Global Arguments stm_exit _ _.
 
   End Statements.
 
-  Section PatternMatching.
+  Fixpoint abstract (Δ : Ctx Set) (τ : Type) {struct Δ} : Type :=
+    match Δ with
+    | ctx_nil => τ
+    | ctx_snoc Δ σ => abstract Δ (σ -> τ)
+    end.
 
-    Fixpoint tuple_pattern_match {σs : Ctx Ty} {Δ : Ctx (𝑿 * Ty)}
-             (p : TuplePat σs Δ) {struct p} : Env TaggedLit σs -> LocalStore Δ :=
-      match p with
-      | tuplepat_nil => fun _ => env_nil
-      | tuplepat_snoc p x =>
-        fun E =>
-          env_snoc
-            (tuple_pattern_match p (env_tail E)) (x, _)
-            (untag (env_lookup E inctx_zero))
-      end.
-
-    Fixpoint record_pattern_match {rfs : Ctx (𝑹𝑭 * Ty)}  {Δ : Ctx (𝑿 * Ty)}
-             (p : RecordPat rfs Δ) {struct p} : Env' TaggedLit rfs -> LocalStore Δ :=
-      match p with
-      | recordpat_nil => fun _ => env_nil
-      | recordpat_snoc p rf x =>
-        fun E =>
-          env_snoc
-            (record_pattern_match p (env_tail E)) (x, _)
-            (untag (env_lookup E inctx_zero))
-      end.
-
-  End PatternMatching.
+  Fixpoint apply {Δ : Ctx Set} {τ : Type} (f : abstract Δ τ) (δ : Env Lit Δ) {struct Δ} : τ :=
+   match Δ return (Env Lit Δ -> abstract Δ τ -> τ) with
+   | ctx_nil => fun _ v => v
+   | ctx_snoc Δ b => fun δ (f : abstract _ (b -> τ)) => apply f (fst δ) (snd δ)
+   end δ f.
 
   (* Record FunDef (Δ : Ctx (𝑿 * Ty)) (τ : Ty) : Set := *)
   (*   { fun_body : Stm Δ τ }. *)
 
-  Module NameResolution.
-
-    Fixpoint ctx_resolve {D : Set} (Γ : Ctx (𝑿 * D)) (x : 𝑿) {struct Γ} : option D :=
-      match Γ with
-      | ctx_nil           => None
-      | ctx_snoc Γ (y, d) => if 𝑿_eq_dec x y then Some d else ctx_resolve Γ x
-      end.
-
-    Definition IsSome {D : Set} (m : option D) : Set :=
-      match m with
-        | Some _ => unit
-        | None => Empty_set
-      end.
-
-    Definition fromSome {D : Set} (m : option D) : IsSome m -> D :=
-      match m return IsSome m -> D with
-      | Some d => fun _ => d
-      | None   => fun p => match p with end
-      end.
-
-    Fixpoint mk_inctx {D : Set} (Γ : Ctx (prod 𝑿 D)) (x : 𝑿) {struct Γ} :
-      let m := ctx_resolve Γ x in forall (p : IsSome m), InCtx (x , fromSome m p) Γ :=
-      match Γ with
-      | ctx_nil => fun p => match p with end
-      | ctx_snoc Γ (y, d) =>
-        match 𝑿_eq_dec x y as s
-        return (forall p, InCtx (x, fromSome (if s then Some d else ctx_resolve Γ x) p)
-                                (ctx_snoc Γ (y, d)))
-        with
-        | left e => fun _ => match e with | eq_refl => inctx_zero end
-        | right _ => fun p => inctx_succ (mk_inctx Γ x p)
-        end
-      end.
-
-    (* Ideally the following smart constructors would perform name resolution
-       and fill in the de Bruijn index and the type of a variable. Unfortunately,
-       they critically rely on the order that type-checking is performed. For
-       instance in context Γ := (ε ▻ ("x", ty_int)) the expression
-       (@exp_smart_var Γ "x" tt) type-checks while the (@exp_smart_var _ "x" tt)
-       fails to type-check with error message
-
-         The term "tt" has type "unit" while it is expected
-         to have type "IsSome (ctx_resolve ?Γ0 "x")".
-
-       So the variable ?Γ0 has not been unified and blocks the evaluation of
-       ctx_resolve. Unfortunately, Coq decides to fail immediately.
-     *)
-    Definition exp_smart_var {Γ : Ctx (𝑿 * Ty)} (x : 𝑿) {p : IsSome (ctx_resolve Γ x)} :
-      Exp Γ (fromSome (ctx_resolve Γ x) p) :=
-      @exp_var Γ x (fromSome (ctx_resolve Γ x) p) (mk_inctx Γ x p).
-
-    Definition stm_smart_assign {Γ : Ctx (𝑿 * Ty)} (x : 𝑿) {p : IsSome (ctx_resolve Γ x)} :
-      Exp Γ (fromSome (ctx_resolve Γ x) p) -> Stm Γ (fromSome (ctx_resolve Γ x) p) :=
-      @stm_assign Γ x (fromSome _ p) (mk_inctx Γ x p).
-
-    (* Instead we hook mk_inctx directly into the typeclass resolution mechanism.
-       Apparently, the unification of Γ is performed before the resolution so
-       evaluation of ctx_resolve and mk_inctx is not blocked.
-     *)
-    Hint Extern 10 (InCtx (?x , _) ?Γ) => exact (mk_inctx Γ x tt) : typeclass_instances.
-
-  End NameResolution.
-
   Section Contracts.
 
-    Definition Pred (A : Set) : Type := A -> Prop.
+    Definition Pred (A : Type) : Type := A -> Prop.
 
-    Definition Final {Γ σ} (s : Stm Γ σ) : Prop :=
+    Definition Final {σ} (s : Stm σ) : Prop :=
       match s with
-      | stm_lit _ _  => True
+      | stm_lit _  => True
       | stm_exit _ _ => True
       | _ => False
       end.
 
     (* Version that computes *)
-    Definition IsLit {Γ σ} (δ : LocalStore Γ) (s : Stm Γ σ) :
-      forall (POST : Lit σ -> Pred (LocalStore Γ)), Prop :=
+    Definition IsLit {σ} (s : Stm σ) :
+      forall (POST : Pred σ), Prop :=
       match s with
-      | stm_lit _ v => fun POST => POST v δ
+      | stm_lit v => fun POST => POST v
       | _ => fun _ => False
       end.
 
-    Lemma IsLit_inversion {Γ σ} (δ : LocalStore Γ) (s : Stm Γ σ)
-          (POST : Lit σ -> Pred (LocalStore Γ)) :
-      IsLit δ s POST -> exists v, s = stm_lit _ v /\ POST v δ.
+    Lemma IsLit_inversion {σ} (s : Stm σ) (POST : Pred σ) :
+      IsLit s POST -> exists v, s = stm_lit v /\ POST v.
     Proof. destruct s; cbn in *; try contradiction; eauto. Qed.
 
-    Record Contract (Δ : Ctx (𝑿 * Ty)) (τ : Ty) : Type :=
-      { contract_pre_condition  : Pred (Env' Lit Δ);
-        contract_post_condition : Lit τ -> Pred (Env' Lit Δ)
-      }.
+    Inductive Contract (Δ : Ctx Set) (τ : Set) : Type :=
+    | ContractWLP (pre : abstract Δ Prop) (post: abstract Δ (τ -> Prop))
+    | ContractWP  (pre : abstract Δ Prop) (post: abstract Δ (τ -> Prop))
+    | ContractNone.
 
     Definition ContractEnv : Type :=
-      forall Δ τ (f : 𝑭 Δ τ), option (Contract Δ τ).
+      forall Δ τ (f : 𝑭 Δ τ), Contract Δ τ.
 
   End Contracts.
 
@@ -561,20 +155,18 @@ End Terms.
 (******************************************************************************)
 
 Module Type ProgramKit
-       (Import typekit : TypeKit)
-       (Import termkit : TermKit typekit).
-  Module TM := Terms typekit termkit.
+       (Import termkit : TermKit).
+  Module TM := Terms termkit.
   Export TM.
 
   (* Parameter Inline Pi : forall {Δ τ} (f : 𝑭 Δ τ), FunDef Δ τ. *)
-  Parameter Inline Pi : forall {Δ τ} (f : 𝑭 Δ τ), Stm Δ τ.
+  Parameter Inline Pi : forall {Δ τ} (f : 𝑭 Δ τ), abstract Δ (Stm τ).
 
 End ProgramKit.
 
 Module Type ContractKit
-       (Import typekit : TypeKit)
-       (Import termkit : TermKit typekit)
-       (Import progkit : ProgramKit typekit termkit).
+       (Import termkit : TermKit)
+       (Import progkit : ProgramKit termkit).
 
   Parameter Inline CEnv : ContractEnv.
 
