test/Example.v
@@ -31,7 +31,15 @@ From Coq Require Import
      Program.Tactics
      Strings.String
      ZArith.ZArith
-     micromega.Lia.
+     micromega.Lia
+     Bool
+     Setoid.
+
+(* Unset SsrRewrite. *)
+(* From Coq Require Import ssreflect ssrfun ssrbool. *)
+(* Set Implicit Arguments. *)
+(* Unset Strict Implicit. *)
+(* Unset Printing Implicit Defensive. *)
 
 From MicroSail Require Import
      WLP.Spec
@@ -39,153 +47,94 @@ From MicroSail Require Import
 
 Set Implicit Arguments.
 Import CtxNotations.
-Import EnvNotations.
 Open Scope string_scope.
 Open Scope Z_scope.
 Open Scope ctx_scope.
-
-Inductive Enums : Set :=
-| ordering.
 
 Inductive Ordering : Set :=
 | LT
 | EQ
 | GT.
 
-Module ExampleTypeKit <: TypeKit.
+Program Instance blastable_ordering : Blastable Ordering :=
+  { blast := fun ord k =>
+               (ord = LT -> k LT) /\
+               (ord = EQ -> k EQ) /\
+               (ord = GT -> k GT) }.
+Solve All Obligations with intros []; intuition; congruence.
 
-  Definition 𝑬 : Set := Enums.
-  Definition 𝑻 : Set := Empty_set.
-  Definition 𝑹 : Set := Empty_set.
-  Definition 𝑿 : Set := string.
-  Definition 𝑿_eq_dec := string_dec.
-
-End ExampleTypeKit.
-Module ExampleTypes := Types ExampleTypeKit.
-Import ExampleTypes.
-
-Notation "x ∶ τ" := (pair x τ) (at level 90, no associativity) : ctx_scope.
 Notation "[ x ]" := (ctx_snoc ctx_nil x) : ctx_scope.
 Notation "[ x , .. , z ]" := (ctx_snoc .. (ctx_snoc ctx_nil x) .. z) : ctx_scope.
 
-Module ExampleTermKit <: (TermKit ExampleTypeKit).
-  Module TY := ExampleTypes.
+Module ExampleTermKit <: TermKit.
 
-  (* Names of union data constructors. *)
-  Definition 𝑬𝑲 (E : 𝑬) : Set :=
-    match E with
-    | ordering => Ordering
-    end.
+  (* Global names and types of functions. *)
+  Inductive Fun : Ctx Set -> Set -> Set :=
+  | abs        : [ Z ]    --> Z
+  | gcd        : [ Z, Z ] --> Z
+  | gcdpos     : [ Z, Z ] --> Z
+  | gcdcompare : [ Z, Z ] --> Z
+  | compare    : [ Z, Z ] --> Ordering
+  where "Γ --> σ" := (Fun Γ σ).
 
-  Definition 𝑲 (T : 𝑻) : Set := match T with end.
-  Definition 𝑲_Ty (T : 𝑻) : 𝑲 T -> Ty := match T with end.
-  Definition 𝑹𝑭  : Set := Empty_set.
-  Definition 𝑹𝑭_Ty (R : 𝑹) : Ctx (𝑹𝑭 * Ty) := match R with end.
-
-  (* Names of functions. *)
-  Inductive Fun : Ctx (𝑿 * Ty) -> Ty -> Set :=
-  | swappair   : Fun
-                   [ "x" ∶ ty_prod ty_bool ty_int ]
-                   (ty_prod ty_int ty_bool)
-  | swaptuple  : Fun
-                   [ "x" ∶ ty_tuple [ ty_bool, ty_int ] ]
-                   (ty_tuple [ ty_int , ty_bool ])
-  | cycletuple : Fun
-                   [ "x" ∶ ty_tuple [ ty_bool, ty_int, ty_string ]]
-                   (ty_tuple [ ty_int, ty_string, ty_bool ])
-  | abs : Fun [ "x" ∶ ty_int ] ty_int
-  | gcd : Fun [ "p" ∶ ty_int, "q" ∶ ty_int ] ty_int
-  | gcdpos : Fun [ "p" ∶ ty_int, "q" ∶ ty_int ] ty_int
-  | gcdcompare : Fun [ "p" ∶ ty_int, "q" ∶ ty_int ] ty_int
-  | compare : Fun [ "x" ∶ ty_int, "y" ∶ ty_int ] (ty_enum ordering)
-  .
-
-  Definition 𝑭  : Ctx (𝑿 * Ty) -> Ty -> Set := Fun.
+  Definition 𝑭  : Ctx Set -> Set -> Set := Fun.
 
 End ExampleTermKit.
-Module ExampleTerms := Terms ExampleTypeKit ExampleTermKit.
+Module ExampleTerms := Terms ExampleTermKit.
 Import ExampleTerms.
-Import NameResolution.
 
+(* Notation "[ x , .. , z ]" := *)
+(*   (tuplepat_snoc .. (tuplepat_snoc tuplepat_nil x) .. z) : pat_scope. *)
 Notation "[ x , .. , z ]" :=
-  (tuplepat_snoc .. (tuplepat_snoc tuplepat_nil x) .. z) : pat_scope.
-Notation "[ x , .. , z ]" :=
-  (env_snoc .. (env_snoc env_nil _ x) .. _ z) : exp_scope.
+  (pair .. (pair tt x) .. z) : exp_scope.
+Notation "'call' f x .. z" :=
+  (stm_app f (pair .. (pair tt x) .. z)) (at level 40, x at next level, z at next level) : exp_scope.
 
-Notation "e1 * e2" := (exp_times e1 e2) : exp_scope.
-Notation "e1 - e2" := (exp_minus e1 e2) : exp_scope.
-Notation "e1 < e2" := (exp_lt e1 e2) : exp_scope.
-Notation "e1 > e2" := (exp_gt e1 e2) : exp_scope.
-Notation "e1 <= e2" := (exp_le e1 e2) : exp_scope.
-Notation "e1 = e2" := (exp_eq e1 e2) : exp_scope.
-Notation "'lit_int' l" := (exp_lit _ ty_int l) (at level 1, no associativity) : exp_scope.
-Notation "'lit_unit'" := (exp_lit _ ty_unit tt) (at level 1, no associativity) : exp_scope.
+Notation "Γ --> σ" := (Fun Γ σ).
+Notation "Γ '-->>' τ" := (abstract Γ τ) (at level 60, right associativity) : type_scope.
+Notation "'if' b 'then' t 'else' f" := (stm_if b%bool t f) (at level 200) : exp_scope.
 
-Local Coercion stmexp := @stm_exp.
 
-Module ExampleProgramKit <: (ProgramKit ExampleTypeKit ExampleTermKit).
+Local Coercion stm_lit_Z := (@stm_lit Z).
+Local Coercion stm_lit_Ordering := (@stm_lit Ordering).
+
+Module ExampleProgramKit <: (ProgramKit ExampleTermKit).
   Module TM := ExampleTerms.
 
   Local Open Scope exp_scope.
 
-  Definition Pi {Δ τ} (f : Fun Δ τ) : Stm Δ τ :=
-    match f in Fun Δ τ return Stm Δ τ with
-    | swappair =>
-      stm_bind
-        (exp_var "x")
-        (fun x : Lit (ty_prod ty_bool ty_int) =>
-           let (l , r) := x in exp_lit _ (ty_prod ty_int ty_bool) (r , l)
-        )
-      (* stm_match_pair (exp_var "x") "l" "r" (exp_pair (exp_var "r") (exp_var "l")) *)
-    | swaptuple => stm_match_tuple (exp_var "x") ["l", "r"] (exp_tuple [exp_var "r", exp_var "l"])
-    | cycletuple => stm_match_tuple
-                      (exp_var "x")
-                      ["u", "v", "w"]
-                      (exp_tuple [exp_var "v", exp_var "w", exp_var "u"])
-    | abs =>
-      stm_if
-        (lit_int (0%Z) <= exp_var "x")
-        (exp_var "x")
-        (exp_neg (exp_var "x"))
-    | gcdcompare =>
-      stm_bind
-        (stm_app compare [exp_var "p", exp_var "q"])
-        (fun K =>
-           match K with
-           | LT => stm_app gcd (env_snoc (env_snoc env_nil ("p" , ty_int) (exp_var "p")) ("q" , ty_int) (exp_var "q" - exp_var "p"))
-           | EQ => stm_exp (exp_var "p")
-           | GT => stm_app gcd (env_snoc (env_snoc env_nil ("p" , ty_int) (exp_var "p" - exp_var "q")) ("q" , ty_int) (exp_var "q"))
-           end)
-      (* stm_let "ord" (ty_enum ordering) *)
-      (*   (stm_app compare [exp_var "p", exp_var "q"]) *)
-      (*   (stm_match_enum ordering (exp_var "ord") *)
-      (*      (fun K => *)
-      (*         match K with *)
-      (*         | LT => stm_app gcd (env_snoc (env_snoc env_nil ("p" , ty_int) (exp_var "p")) ("q" , ty_int) (exp_var "q" - exp_var "p")) *)
-      (*         | EQ => stm_exp (exp_var "p") *)
-      (*         | GT => stm_app gcd (env_snoc (env_snoc env_nil ("p" , ty_int) (exp_var "p" - exp_var "q")) ("q" , ty_int) (exp_var "q")) *)
-      (*         end)) *)
-    | gcd =>
-      stm_let "p'" ty_int (stm_app abs [exp_var "p"])
-      (stm_let "q'" ty_int (stm_app abs [exp_var "q"])
-        (stm_app gcdpos [exp_var "p'", exp_var "q'"]))
-    | gcdpos =>
-      stm_if
-        (exp_var "p" = exp_var "q")
-        (exp_var "p")
-        (stm_if
-           (exp_var "p" < exp_var "q")
-           (stm_app gcd (env_snoc (env_snoc env_nil ("p" , ty_int) (exp_var "p")) ("q" , ty_int) (exp_var "q" - exp_var "p")))
-           (stm_app gcd (env_snoc (env_snoc env_nil ("p" , ty_int) (exp_var "p" - exp_var "q")) ("q" , ty_int) (exp_var "q")))
-        )
-    | compare =>
-      stm_if (exp_var "x" < exp_var "y")
-        (stm_lit (ty_enum ordering) LT)
-      (stm_if (exp_var "x" = exp_var "y")
-        (stm_lit (ty_enum ordering) EQ)
-      (stm_if (exp_var "x" > exp_var "y")
-        (stm_lit (ty_enum ordering) GT)
-        (stm_exit (ty_enum ordering) "compare")))
+  Local Notation "ma >>= f" := (stm_bind ma f) (at level 50, left associativity).
+  (* Notation "ma *> mb" := (bindright ma mb) (at level 50, left associativity). *)
+  (* Notation "ma <* mb" := (bindleft ma mb) (at level 50, left associativity). *)
+
+  Definition Pi {Δ τ} (f : Δ --> τ) : Δ -->> Stm τ :=
+    match f with
+    | abs => fun x => if 0 <=? x then x else (- x)
+    | gcd => fun p q =>
+               stm_app abs [p] >>= fun p' =>
+               stm_app abs [q] >>= fun q' =>
+               if (0 <? p') && (0 <? q')
+               then stm_app gcdpos [p', q']
+               else p' + q'
+    | gcdpos => fun p q =>
+                  if p =? q then
+                    p
+                  else if p <? q then
+                    stm_app gcdpos [p, q - p]
+                  else
+                    stm_app gcdpos [p - q, q]
+    | gcdcompare => fun p q =>
+                      stm_app compare [p, q] >>= fun ord =>
+                      match ord with
+                      | LT => stm_app gcdcompare [p, q - p]
+                      | EQ => p
+                      | GT => stm_app gcdcompare [p - q, q]
+                      end
+    | compare => fun x y =>
+                   if x <? y then LT else
+                   if x =? y then EQ else
+                   if x >? y then GT else
+                   stm_exit Ordering "compare"
     end.
 
 End ExampleProgramKit.
@@ -193,97 +142,92 @@ Import ExampleProgramKit.
 
 (******************************************************************************)
 
-Module ExampleContractKit <: (ContractKit ExampleTypeKit ExampleTermKit ExampleProgramKit).
+Module ExampleContractKit <: (ContractKit ExampleTermKit ExampleProgramKit).
 
   Definition CEnv : ContractEnv :=
-    fun σs τ f =>
+    fun (σs : Ctx Set) (τ : Set) (f : Fun σs τ) =>
       match f with
-      | abs =>
-        Some {| contract_pre_condition := fun _ => True;
-                contract_post_condition := fun (v : Lit ty_int)
-                                               (δ : Env' Lit [ "x" ∶ ty_int ]) =>
-                                             v = Z.abs (δ ! "x")
-             |}
-      | compare =>
-        Some {| contract_pre_condition := fun _ => True;
-                contract_post_condition := fun (K : Lit (ty_enum ordering))
-                                               (δ : Env' Lit [ "x" ∶ ty_int , "y" ∶ ty_int ]) =>
-                                             match K with
-                                             | LT => δ ! "x" <= δ ! "y"
-                                             | EQ => δ ! "x"  = δ ! "y"
-                                             | GT => δ ! "x" >= δ ! "y"
-                                             end
-             |}
-      | gcdpos =>
-        Some {| contract_pre_condition := fun (δ : Env' Lit [ "p" ∶ ty_int , "q" ∶ ty_int ]) =>
-                                            (δ ! "p") >= 0 /\ (δ ! "q" >= 0);
-                contract_post_condition := fun (r : Lit ty_int)
-                                               (δ : Env' Lit [ "p" ∶ ty_int , "q" ∶ ty_int ]) =>
-                                             r = Z.gcd (δ ! "p") (δ ! "q")
-             |}
-      | gcd =>
-        Some {| contract_pre_condition := fun (δ : Env' Lit [ "p" ∶ ty_int , "q" ∶ ty_int ]) => True;
-                contract_post_condition := fun (r : Lit ty_int)
-                                               (δ : Env' Lit [ "p" ∶ ty_int , "q" ∶ ty_int ]) =>
-                                             r = Z.gcd (δ ! "p") (δ ! "q")
-             |}
-      | _ => Some {| contract_pre_condition := fun _ => True;
-                     contract_post_condition := fun _ _ => True
-                  |}
+      | abs        => ContractWLP [Z] Z
+                        (fun _ => True)
+                        (fun x r => r = Z.abs x)
+      | gcdpos     => ContractWLP [Z, Z] Z
+                        (fun p q => p > 0 /\ q > 0)
+                        (fun p q r => r = Z.gcd p q)
+      | compare    => ContractWLP [Z, Z] Ordering
+                        (fun _ _ => True)
+                        (fun x y ord =>
+                           (x < y <-> ord = LT) /\
+                           (x = y <-> ord = EQ) /\
+                           (x > y <-> ord = GT)
+                           (* match ord with *)
+                           (* | LT => x < y *)
+                           (* | EQ => x = y *)
+                           (* | GT => x > y *)
+                           (* end *)
+                        )
+      | gcd        => ContractWLP [Z, Z] Z
+                        (fun _ _ => True)
+                        (fun p q r => r = Z.gcd p q)
+      | gcdcompare => ContractWLP [Z, Z] Z
+                        (fun p q => p > 0 /\ q > 0)
+                        (fun p q r => r = Z.gcd p q)
       end.
 
 End ExampleContractKit.
 Import ExampleContractKit.
 
-Module ExampleWLP := WLP ExampleTypeKit ExampleTermKit ExampleProgramKit ExampleContractKit.
+Module ExampleWLP := WLP ExampleTermKit ExampleProgramKit ExampleContractKit.
 Import ExampleWLP.
 
-Definition ValidContract {Γ τ} (c : Contract Γ τ) (s : Stm Γ τ) : Prop :=
-  forall δ, contract_pre_condition c δ -> WLP s (contract_post_condition c) δ.
+Fixpoint Forall (Δ : Ctx Set) {struct Δ} : (Env Lit Δ -> Prop) -> Prop :=
+  match Δ return (Env Lit Δ -> Prop) -> Prop with
+  | ctx_nil      => fun P => P tt
+  | ctx_snoc Δ b => fun P => Forall Δ (fun δ => forall v, P (δ, v))
+  end.
+
+Definition ValidContract {Γ τ} (c : Contract Γ τ) (s : abstract Γ (Stm τ)) : Prop :=
+  match c with
+  | ContractWLP _ _ pre post => Forall Γ (fun δ => apply pre δ -> WLP (apply s δ) (apply post δ))
+  | _ => True
+  end.
 
 Definition ValidContractEnv (cenv : ContractEnv) : Prop :=
-  forall σs σ (f : 𝑭 σs σ),
-    match cenv σs σ f with
-    | Some c => ValidContract c (Pi f)
-    | None => True
-    end.
+  forall σs σ (f : 𝑭 σs σ), ValidContract (cenv σs σ f) (Pi f).
 
 Lemma gcd_sub_diag_l (n m : Z) : Z.gcd (n - m) m = Z.gcd n m.
 Proof. now rewrite Z.gcd_comm, Z.gcd_sub_diag_r, Z.gcd_comm. Qed.
 
+Lemma abs_le_0 (n : Z) :
+  Z.abs n <= 0 <-> n = 0.
+Proof. lia. Qed.
+
 Ltac validate_destr :=
   match goal with
-  | [ |- _ -> _ ]  => intro
-  | [ |- True ]  => constructor
   | [ H: True |- _ ] => clear H
   | [ H: False |- _ ] => destruct H
-  | [ H: Env _ (ctx_snoc _ _) |- _ ] => dependent destruction H
-  | [ H: Env _ ctx_nil |- _ ] => dependent destruction H
-  | [ H: Env' _ (ctx_snoc _ _) |- _ ] => dependent destruction H
-  | [ H: Env' _ ctx_nil |- _ ] => dependent destruction H
+  | [ |- _ -> _ ]  => intro
+  | [ |- True ]  => constructor
   end.
 
 Ltac validate_simpl :=
   repeat
-    (cbn in *; repeat validate_destr; destruct_conjs; subst;
-     rewrite ?Z.eqb_eq, ?Z.eqb_neq, ?Z.leb_gt, ?Z.ltb_ge, ?Z.ltb_lt, ?Z.leb_le, ?Z.gtb_ltb,
-       ?Z.gcd_diag, ?Z.gcd_abs_l, ?Z.gcd_abs_r, ?Z.gcd_sub_diag_r, ?gcd_sub_diag_l in *).
+    (cbn in *; repeat validate_destr; destruct_conjs; subst; try discriminate;
+     rewrite ?andb_true_iff, ?andb_false_iff, ?abs_le_0, ?Z.eqb_eq, ?Z.eqb_neq, ?Z.leb_gt, ?Z.ltb_ge, ?Z.ltb_lt, ?Z.leb_le, ?Z.gtb_ltb,
+       ?Z.gcd_diag, ?Z.gcd_abs_l, ?Z.gcd_abs_r, ?Z.gcd_sub_diag_r, ?Z.gcd_0_r, ?Z.gcd_0_l, ?gcd_sub_diag_l in *).
 
+     (* ?andb_false_iff, *)
 Ltac validate_case :=
   match goal with
-  | [ |- match ?e with _ => _ end _ _ ] =>
+  | [ |- match ?e with _ => _ end _ ] =>
     case_eq e
-  | [ |- WLP match ?e with _ => _ end _ _ ] =>
+  | [ |- WLP match ?e with _ => _ end _ ] =>
     case_eq e
   end.
 
 Ltac validate_solve :=
-  repeat
-    (validate_simpl; intuition;
-     try lia;
-     try validate_case).
+  repeat (validate_simpl; intuition; try lia).
 
 Lemma validCEnv : ValidContractEnv CEnv.
-Proof. intros σs τ [] δ; validate_solve. Qed.
+Proof. time (intros σs τ [] δ; validate_solve). Qed.
 
-(* Print Assumptions validCEnv. *)
+Print Assumptions validCEnv.
