src/MicroSail/Environment.v
@@ -5,139 +5,160 @@ Require Import MicroSail.Notation.
 Set Implicit Arguments.
 
 Section WithBinding.
-  Context {B : Set}.
+  Context {B : Type}.
 
-  Inductive Env (D : B -> Set) : Ctx B -> Set :=
-  | env_nil : Env D ctx_nil
-  | env_snoc {Γ} (E : Env D Γ) (b : B) (db : D b) :
-      Env D (ctx_snoc Γ b).
-
-  Global Arguments env_nil {_}.
+  Fixpoint Env (D : B -> Type) (Γ : Ctx B) : Type :=
+    match Γ with
+    | ctx_nil => unit
+    | ctx_snoc Γ x => prod (Env D Γ) (D x)
+    end.
+  (* Global Arguments env_nil {_}. *)
   Bind Scope env_scope with Env.
 
-  Fixpoint env_cat {D : B -> Set} {Γ Δ : Ctx B}
-    (EΓ : Env D Γ) (EΔ : Env D Δ) : Env D (ctx_cat Γ Δ) :=
-    match EΔ with
-    | env_nil => EΓ
-    | env_snoc E b db => env_snoc (env_cat EΓ E) b db
+  Fixpoint Env_ind (D : B -> Type) (P : forall Γ, Env D Γ -> Prop)
+    (en : P ctx_nil tt)
+    (ec : forall Γ E, P Γ E -> forall x (d : D x), P (ctx_snoc Γ x) (E , d))
+    (Γ : Ctx B) {struct Γ} : forall (E : Env D Γ), P Γ E :=
+    match Γ with
+    | ctx_nil => fun E => match E with | tt => en end
+    | ctx_snoc Γ b =>
+      fun EΓb =>
+        match EΓb with
+        | (EΓ , db) => ec Γ EΓ (Env_ind D P en ec Γ EΓ) b db
+        end
     end.
 
-  Fixpoint env_map {D1 D2 : B -> Set} {Γ : Ctx B}
-    (f : forall b, D1 b -> D2 b) (E : Env D1 Γ) : Env D2 Γ :=
-    match E with
-    | env_nil => env_nil
-    | env_snoc E b db => env_snoc (env_map f E) b (f b db)
-    end.
+  (* Inductive Env (D : B -> Type) : Ctx B -> Type := *)
+  (* | env_nil : Env D ctx_nil *)
+  (* | env_snoc {Γ} (E : Env D Γ) (b : B) (db : D b) : *)
+  (*     Env D (ctx_snoc Γ b). *)
 
-  Fixpoint env_lookup {D : B -> Set} {Γ : Ctx B}
-    (E : Env D Γ) : forall (b : B) (bIn : InCtx b Γ), D b :=
-    match E with
-    | env_nil => fun _ => inctx_case_nil
-    | env_snoc E b db => inctx_case_snoc D db (env_lookup E)
-    end.
+  (* Global Arguments env_nil {_}. *)
+  (* Bind Scope env_scope with Env. *)
 
-  Global Arguments env_lookup {_ _} _ [_] _.
-
-  Fixpoint env_update {D : B -> Set} {Γ : Ctx B} (E : Env D Γ) {struct E} :
-    forall {b0 : B} (bIn0 : InCtx b0 Γ) (new : D b0), Env D Γ :=
-    match E with
-    | env_nil => fun _ => inctx_case_nil
-    | @env_snoc _ Γ E b bold =>
-      inctx_case_snoc
-        (fun z => D z -> Env D (ctx_snoc Γ b))
-        (fun new => env_snoc E b new)
-        (fun b0' bIn0' new => env_snoc (env_update E bIn0' new) b bold)
-    end.
-
-  Definition env_tail {D : B -> Set} {Γ : Ctx B}
-    {b : B} (E : Env D (ctx_snoc Γ b)) : Env D Γ :=
-    match E in Env _ Γb
-    return match Γb with
-           | ctx_nil => unit
-           | ctx_snoc Γ _ => Env D Γ
-           end
-    with
-      | env_nil => tt
-      | env_snoc E _ _ => E
-    end.
-
-  Global Arguments env_tail {_ _ _} / _.
-
-  Fixpoint env_drop {D : B -> Set} {Γ : Ctx B} Δ {struct Δ} :
-    forall (E : Env D (ctx_cat Γ Δ)), Env D Γ :=
+  Fixpoint env_cat {D : B -> Type} {Γ Δ : Ctx B} (EΓ : Env D Γ) {struct Δ} :
+    Env D Δ -> Env D (ctx_cat Γ Δ) :=
     match Δ with
-    | ctx_nil => fun E => E
-    | ctx_snoc Δ _ => fun E => env_drop Δ (env_tail E)
+    | ctx_nil => fun EΔ => EΓ
+    | ctx_snoc Δ b => fun EΔ => (env_cat EΓ (fst EΔ), snd EΔ)
     end.
 
-  Fixpoint env_split {D : B -> Set} {Γ : Ctx B} Δ {struct Δ} :
-    forall (E : Env D (ctx_cat Γ Δ)), Env D Γ * Env D Δ :=
-    match Δ with
-    | ctx_nil => fun E => (E , env_nil)
-    | ctx_snoc Δ b =>
-      fun E =>
-        match E in (Env _ ΓΔb)
-        return match ΓΔb with
-               | ctx_nil => unit
-               | ctx_snoc ΓΔ b => (Env D ΓΔ -> Env D Γ * Env D Δ) ->
-                                  Env D Γ * Env D (ctx_snoc Δ b)
-               end
-        with
-        | env_nil => tt
-        | env_snoc EΓΔ b db =>
-          fun split => let (EΓ, EΔ) := split EΓΔ in (EΓ, env_snoc EΔ b db)
-        end (env_split Δ)
-    end.
+  (* Fixpoint env_map {D₁ D₂ : B -> Type} {Γ : Ctx B} *)
+  (*          (f : forall x, D₁ x -> D₂ x) {struct Γ} : Env D₁ Γ -> Env D₂ Γ := *)
+  (*   match Γ as c return (Env D₁ c -> Env D₂ c) with *)
+  (*   | ctx_nil => fun E => E *)
+  (*   | ctx_snoc Γ b => fun EΓb => (env_map f (fst EΓb), f b (snd EΓb)) *)
+  (*   end. *)
 
-  Lemma env_lookup_update {D : B -> Set} {Γ : Ctx B} (E : Env D Γ) :
-    forall {b : B} (bInΓ : InCtx b Γ) (db : D b),
-      env_lookup (env_update E bInΓ db) bInΓ = db.
-  Proof.
-    induction E; intros ? [n e]; try destruct e;
-      destruct n; cbn in *; subst; auto.
-  Qed.
+  (* Fixpoint env_lookup {D : B -> Type} {Γ : Ctx B} *)
+  (*   (E : Env D Γ) : forall (b : B) (bIn : InCtx b Γ), D b := *)
+  (*   match E with *)
+  (*   | env_nil => fun _ => inctx_case_nil *)
+  (*   | env_snoc E b db => inctx_case_snoc D db (env_lookup E) *)
+  (*   end. *)
 
-  Lemma env_split_cat {D : B -> Set} {Γ Δ : Ctx B} :
-    forall (EΓ : Env D Γ) (EΔ : Env D Δ),
-      env_split Δ (env_cat EΓ EΔ) = (EΓ , EΔ).
-  Proof. induction EΔ using Env_ind; cbn; now try rewrite IHEΔ. Qed.
+  (* Global Arguments env_lookup {_ _} _ [_] _. *)
 
-  Lemma env_cat_split' {D : B -> Set} {Γ Δ : Ctx B} :
-    forall (EΓΔ : Env D (ctx_cat Γ Δ)),
-      let (EΓ,EΔ) := env_split _ EΓΔ in
-      EΓΔ = env_cat EΓ EΔ.
-  Proof.
-    induction Δ; intros; cbn in *.
-    - reflexivity.
-    - dependent destruction EΓΔ.
-      specialize (IHΔ EΓΔ); cbn in *.
-      destruct (env_split Δ EΓΔ); now subst.
-  Qed.
+  (* Fixpoint env_update {D : B -> Type} {Γ : Ctx B} (E : Env D Γ) {struct E} : *)
+  (*   forall {b0 : B} (bIn0 : InCtx b0 Γ) (new : D b0), Env D Γ := *)
+  (*   match E with *)
+  (*   | env_nil => fun _ => inctx_case_nil *)
+  (*   | @env_snoc _ Γ E b bold => *)
+  (*     inctx_case_snoc *)
+  (*       (fun z => D z -> Env D (ctx_snoc Γ b)) *)
+  (*       (fun new => env_snoc E b new) *)
+  (*       (fun b0' bIn0' new => env_snoc (env_update E bIn0' new) b bold) *)
+  (*   end. *)
 
-  Lemma env_cat_split {D : B -> Set} {Γ Δ : Ctx B} (EΓΔ : Env D (ctx_cat Γ Δ)) :
-    EΓΔ = env_cat (fst (env_split _ EΓΔ)) (snd (env_split _ EΓΔ)).
-  Proof.
-    generalize (env_cat_split' EΓΔ).
-    now destruct (env_split Δ EΓΔ).
-  Qed.
+  (* Definition env_tail {D : B -> Type} {Γ : Ctx B} *)
+  (*   {b : B} (E : Env D (ctx_snoc Γ b)) : Env D Γ := *)
+  (*   match E in Env _ Γb *)
+  (*   return match Γb with *)
+  (*          | ctx_nil => unit *)
+  (*          | ctx_snoc Γ _ => Env D Γ *)
+  (*          end *)
+  (*   with *)
+  (*     | env_nil => tt *)
+  (*     | env_snoc E _ _ => E *)
+  (*   end. *)
 
-  Lemma env_drop_cat {D : B -> Set} {Γ Δ : Ctx B} :
-    forall (δΔ : Env D Δ) (δΓ : Env D Γ),
-      env_drop Δ (env_cat δΓ δΔ) = δΓ.
-  Proof. induction δΔ; cbn; auto. Qed.
+  (* Global Arguments env_tail {_ _ _} / _. *)
+
+  (* Fixpoint env_drop {D : B -> Type} {Γ : Ctx B} Δ {struct Δ} : *)
+  (*   forall (E : Env D (ctx_cat Γ Δ)), Env D Γ := *)
+  (*   match Δ with *)
+  (*   | ctx_nil => fun E => E *)
+  (*   | ctx_snoc Δ _ => fun E => env_drop Δ (env_tail E) *)
+  (*   end. *)
+
+  (* Fixpoint env_split {D : B -> Type} {Γ : Ctx B} Δ {struct Δ} : *)
+  (*   forall (E : Env D (ctx_cat Γ Δ)), Env D Γ * Env D Δ := *)
+  (*   match Δ with *)
+  (*   | ctx_nil => fun E => (E , env_nil) *)
+  (*   | ctx_snoc Δ b => *)
+  (*     fun E => *)
+  (*       match E in (Env _ ΓΔb) *)
+  (*       return match ΓΔb with *)
+  (*              | ctx_nil => unit *)
+  (*              | ctx_snoc ΓΔ b => (Env D ΓΔ -> Env D Γ * Env D Δ) -> *)
+  (*                                 Env D Γ * Env D (ctx_snoc Δ b) *)
+  (*              end *)
+  (*       with *)
+  (*       | env_nil => tt *)
+  (*       | env_snoc EΓΔ b db => *)
+  (*         fun split => let (EΓ, EΔ) := split EΓΔ in (EΓ, env_snoc EΔ b db) *)
+  (*       end (env_split Δ) *)
+  (*   end. *)
+
+  (* Lemma env_lookup_update {D : B -> Type} {Γ : Ctx B} (E : Env D Γ) : *)
+  (*   forall {b : B} (bInΓ : InCtx b Γ) (db : D b), *)
+  (*     env_lookup (env_update E bInΓ db) bInΓ = db. *)
+  (* Proof. *)
+  (*   induction E; intros ? [n e]; try destruct e; *)
+  (*     destruct n; cbn in *; subst; auto. *)
+  (* Qed. *)
+
+  (* Lemma env_split_cat {D : B -> Type} {Γ Δ : Ctx B} : *)
+  (*   forall (EΓ : Env D Γ) (EΔ : Env D Δ), *)
+  (*     env_split Δ (env_cat EΓ EΔ) = (EΓ , EΔ). *)
+  (* Proof. induction EΔ using Env_ind; cbn; now try rewrite IHEΔ. Qed. *)
+
+  (* Lemma env_cat_split' {D : B -> Type} {Γ Δ : Ctx B} : *)
+  (*   forall (EΓΔ : Env D (ctx_cat Γ Δ)), *)
+  (*     let (EΓ,EΔ) := env_split _ EΓΔ in *)
+  (*     EΓΔ = env_cat EΓ EΔ. *)
+  (* Proof. *)
+  (*   induction Δ; intros; cbn in *. *)
+  (*   - reflexivity. *)
+  (*   - dependent destruction EΓΔ. *)
+  (*     specialize (IHΔ EΓΔ); cbn in *. *)
+  (*     destruct (env_split Δ EΓΔ); now subst. *)
+  (* Qed. *)
+
+  (* Lemma env_cat_split {D : B -> Type} {Γ Δ : Ctx B} (EΓΔ : Env D (ctx_cat Γ Δ)) : *)
+  (*   EΓΔ = env_cat (fst (env_split _ EΓΔ)) (snd (env_split _ EΓΔ)). *)
+  (* Proof. *)
+  (*   generalize (env_cat_split' EΓΔ). *)
+  (*   now destruct (env_split Δ EΓΔ). *)
+  (* Qed. *)
+
+  (* Lemma env_drop_cat {D : B -> Type} {Γ Δ : Ctx B} : *)
+  (*   forall (δΔ : Env D Δ) (δΓ : Env D Γ), *)
+  (*     env_drop Δ (env_cat δΓ δΔ) = δΓ. *)
+  (* Proof. induction δΔ; cbn; auto. Qed. *)
 
 End WithBinding.
 
-Definition Env' {X T : Set} (D : T -> Set) (Γ : Ctx (X * T)) : Set :=
-  Env (fun xt => D (snd xt)) Γ.
+(* Definition Env' {X T : Set} (D : T -> Type) (Γ : Ctx (X * T)) : Type := *)
+(*   Env (fun xt => D (snd xt)) Γ. *)
 Bind Scope env_scope with Env.
-Bind Scope env_scope with Env'.
+(* Bind Scope env_scope with Env'. *)
 
-Module EnvNotations.
+(* Module EnvNotations. *)
 
-  Notation "δ '►' b '↦' d" := (env_snoc δ b d).
-  Notation "δ1 '►►' δ2" := (env_cat δ1 δ2).
-  Notation "δ [ x ↦ v ]" := (@env_update _ _ _ δ (x , _) _ v).
-  Notation "δ ! x" := (@env_lookup _ _ _ δ (x , _) _).
+(*   Notation "δ '►' b '↦' d" := (env_snoc δ b d). *)
+(*   Notation "δ1 '►►' δ2" := (env_cat δ1 δ2). *)
+(*   Notation "δ [ x ↦ v ]" := (@env_update _ _ _ δ (x , _) _ v). *)
+(*   Notation "δ ! x" := (@env_lookup _ _ _ δ (x , _) _). *)
 
-End EnvNotations.
+(* End EnvNotations. *)
