src/MicroSail/SmallStep/Progress.v
@@ -35,29 +35,13 @@ From MicroSail Require Import
 Set Implicit Arguments.
 
 Module Progress
-       (Import typekit : TypeKit)
-       (Import termkit : TermKit typekit)
-       (Import progkit : ProgramKit typekit termkit).
-  Module SS := SmallStep typekit termkit progkit.
+       (Import termkit : TermKit)
+       (Import progkit : ProgramKit termkit).
+  Module SS := SmallStep termkit progkit.
   Import SS.
-
-  Lemma can_form_store_cat (Γ Δ : Ctx (𝑿 * Ty)) (δ : LocalStore (ctx_cat Γ Δ)) :
-    exists (δ1 : LocalStore Γ) (δ2 : LocalStore Δ), δ = env_cat δ1 δ2.
-  Proof. pose (env_cat_split δ); eauto. Qed.
-
-  (* Lemma can_form_store_snoc (Γ : Ctx (𝑿 * Ty)) (x : 𝑿) (σ : Ty) (δ : LocalStore (Γ ▻ (x , σ))) : *)
-  (*   exists (δ' : LocalStore Γ) (v : Lit σ), δ = env_snoc δ' x σ v. *)
-  (* Admitted. *)
-
-  (* Lemma can_form_store_nil (δ : LocalStore ε) : *)
-  (*   δ = env_nil. *)
-  (* Admitted. *)
 
   Local Ltac progress_can_form :=
     match goal with
-    (* | [ H: LocalStore (ctx_snoc _ _) |- _ ] => pose proof (can_form_store_snoc H) *)
-    (* | [ H: LocalStore ctx_nil |- _ ] => pose proof (can_form_store_nil H) *)
-    | [ H: LocalStore (ctx_cat _ _) |- _ ] => pose proof (can_form_store_cat _ _ H)
     | [ H: Final ?s |- _ ] => destruct s; cbn in H
     end; destruct_conjs; subst; try contradiction.
 
@@ -73,27 +57,14 @@ Module Progress
            | [ H : _ \/ _ |- _ ] => destruct H
            end).
 
-  Local Ltac progress_inst T :=
-    match goal with
-    | [ IH: (forall (δ : LocalStore (ctx_cat ?Γ ?Δ)), _),
-        δ1: LocalStore ?Γ, δ2: LocalStore ?Δ |- _
-      ] => specialize (IH (env_cat δ1 δ2)); T
-    (* | [ IH: (forall (δ : LocalStore (ctx_snoc ctx_nil (?x , ?σ))), _), *)
-    (*     v: Lit ?σ |- _ *)
-    (*   ] => specialize (IH (env_snoc env_nil x σ v)); T *)
-    | [ IH: (forall (δ : LocalStore ?Γ), _), δ: LocalStore ?Γ |- _
-      ] => solve [ specialize (IH δ); T | clear IH; T ]
-    end.
-
   Local Ltac progress_tac :=
     progress_simpl;
     solve
       [ repeat eexists; constructor; eauto
-      | progress_inst progress_tac
       ].
 
-  Lemma progress {Γ σ} (s : Stm Γ σ) :
-    Final s \/ forall δ, exists δ' s', ⟨ δ , s ⟩ ---> ⟨ δ' , s' ⟩.
+  Lemma progress {σ} (s : Stm σ) :
+    Final s \/ exists s', s ---> s'.
   Proof. induction s; intros; try progress_tac. Qed.
 
 End Progress.
