src/MicroSail/SmallStep/Step.v
@@ -34,153 +34,60 @@ From MicroSail Require Import
 Set Implicit Arguments.
 
 Module SmallStep
-  (Import typekit : TypeKit)
-  (Import termkit : TermKit typekit)
-  (Import progKit : ProgramKit typekit termkit).
+  (Import termkit : TermKit)
+  (Import progKit : ProgramKit termkit).
 
   Import CtxNotations.
-  Import EnvNotations.
 
-  Inductive Step {Γ : Ctx (𝑿 * Ty)} : forall {σ : Ty} (δ1 δ2 : LocalStore Γ) (s1 s2 : Stm Γ σ), Prop :=
-
-  | step_stm_exp
-      (δ : LocalStore Γ) (σ : Ty) (e : Exp Γ σ) :
-      ⟨ δ , stm_exp e ⟩ ---> ⟨ δ , stm_lit σ (eval e δ) ⟩
-
-  | step_stm_let_value
-      (δ : LocalStore Γ) (x : 𝑿) (τ σ : Ty) (v : Lit τ) (k : Stm (Γ ▻ (x , τ)) σ) :
-      ⟨ δ , stm_let x τ (stm_lit τ v) k ⟩ ---> ⟨ δ , stm_let' (env_snoc env_nil (x,τ) v) k ⟩
-  | step_stm_let_exit
-      (δ : LocalStore Γ) (x : 𝑿) (τ σ : Ty) (s : string) (k : Stm (Γ ▻ (x , τ)) σ) :
-      ⟨ δ , stm_let x τ (stm_exit τ s) k ⟩ ---> ⟨ δ , stm_exit σ s ⟩
-  | step_stm_let_step
-      (δ : LocalStore Γ) (δ' : LocalStore Γ) (x : 𝑿) (τ σ : Ty)
-      (s : Stm Γ τ) (s' : Stm Γ τ) (k : Stm (Γ ▻ (x , τ)) σ) :
-      ⟨ δ , s ⟩ ---> ⟨ δ' , s' ⟩ ->
-      ⟨ δ , stm_let x τ s k ⟩ ---> ⟨ δ' , stm_let x τ s' k ⟩
-  | step_stm_let'_value
-      (δ : LocalStore Γ) (Δ : Ctx (𝑿 * Ty)) (δΔ : LocalStore Δ) (σ : Ty) (v : Lit σ) :
-      ⟨ δ , stm_let' δΔ (stm_lit σ v) ⟩ ---> ⟨ δ , stm_lit σ v ⟩
-  | step_stm_let'_exit
-      (δ : LocalStore Γ) (Δ : Ctx (𝑿 * Ty)) (δΔ : LocalStore Δ) (σ : Ty) (s : string) :
-      ⟨ δ , stm_let' δΔ (stm_exit σ s) ⟩ ---> ⟨ δ , stm_exit σ s ⟩
-  | step_stm_let'_step
-      (δ δ' : LocalStore Γ) (Δ : Ctx (𝑿 * Ty)) (δΔ δΔ' : LocalStore Δ) (σ : Ty) (k k' : Stm (Γ ▻▻ Δ) σ) :
-      ⟨ δ ►► δΔ , k ⟩ ---> ⟨ δ' ►► δΔ' , k' ⟩ ->
-      ⟨ δ , stm_let' δΔ k ⟩ ---> ⟨ δ' , stm_let' δΔ' k' ⟩
-
-  | step_stm_seq_step
-      (δ δ' : LocalStore Γ) (τ σ : Ty) (s s' : Stm Γ τ) (k : Stm Γ σ) :
-      ⟨ δ , s ⟩ ---> ⟨ δ' , s' ⟩ ->
-      ⟨ δ , stm_seq s k ⟩ ---> ⟨ δ' , stm_seq s' k ⟩
-  | step_stm_seq_value
-      (δ : LocalStore Γ) (τ σ : Ty) (v : Lit τ) (k : Stm Γ σ) :
-      ⟨ δ , stm_seq (stm_lit τ v) k ⟩ ---> ⟨ δ , k ⟩
-  | step_stm_seq_exit
-      (δ : LocalStore Γ) (τ σ : Ty) (s : string) (k : Stm Γ σ) :
-      ⟨ δ , stm_seq (stm_exit τ s) k ⟩ ---> ⟨ δ , stm_exit σ s ⟩
+  Inductive Step : forall {σ : Set} (s1 s2 : Stm σ), Prop :=
 
   | step_stm_app
-      {δ : LocalStore Γ} {σs σ} {f : 𝑭 σs σ} (es : Env' (Exp Γ) σs) :
-      ⟨ δ , stm_app f es ⟩ --->
-      ⟨ δ , stm_app' σs (evals es δ) σ (Pi f) ⟩
-  | step_stm_app'_step
-      {δ : LocalStore Γ} (Δ : Ctx (𝑿 * Ty)) {δΔ δΔ' : LocalStore Δ} (τ : Ty)
-      (s s' : Stm Δ τ) :
-      ⟨ δΔ , s ⟩ ---> ⟨ δΔ' , s' ⟩ ->
-      ⟨ δ , stm_app' Δ δΔ τ s ⟩ ---> ⟨ δ , stm_app' Δ δΔ' τ s' ⟩
-  | step_stm_app'_value
-      {δ : LocalStore Γ} (Δ : Ctx (𝑿 * Ty)) {δΔ : LocalStore Δ} (τ : Ty) (v : Lit τ) :
-      ⟨ δ , stm_app' Δ δΔ τ (stm_lit τ v) ⟩ ---> ⟨ δ , stm_lit τ v ⟩
-  | step_stm_app'_exit
-      {δ : LocalStore Γ} (Δ : Ctx (𝑿 * Ty)) {δΔ : LocalStore Δ} (τ : Ty) (s : string) :
-      ⟨ δ , stm_app' Δ δΔ τ (stm_exit τ s) ⟩ ---> ⟨ δ , stm_exit τ s ⟩
-  | step_stm_assign
-      (δ : LocalStore Γ) (x : 𝑿) (σ : Ty) {xInΓ : InCtx (x , σ) Γ} (e : Exp Γ σ) :
-      let v := eval e δ in
-      ⟨ δ , stm_assign x e ⟩ ---> ⟨ δ [ x ↦ v ] , stm_lit σ v ⟩
+      {σs σ} {f : 𝑭 σs σ} (es : Env Lit σs) :
+      stm_app f es --->
+      apply (Pi f) es
   | step_stm_if
-      (δ : LocalStore Γ) (e : Exp Γ ty_bool) (σ : Ty) (s1 s2 : Stm Γ σ) :
-      ⟨ δ , stm_if e s1 s2 ⟩ ---> ⟨ δ , if eval e δ then s1 else s2 ⟩
+      (e : bool) (σ : Set) (s1 s2 : Stm σ) :
+      stm_if e s1 s2 ---> if e then s1 else s2
   | step_stm_assert
-      (δ : LocalStore Γ) (e1 : Exp Γ ty_bool) (e2 : Exp Γ ty_string) :
-      ⟨ δ , stm_assert e1 e2 ⟩ --->
-      ⟨ δ , if eval e1 δ then stm_lit ty_bool true else stm_exit ty_bool (eval e2 δ) ⟩
-  (* | step_stm_while : *)
-  (*   (δ : LocalStore Γ) (w : 𝑾 δ) (e : Exp Γ ty_bool) {σ : Ty} (s : Stm Γ σ) -> *)
-  (*   ⟨ δ , stm_while w e s ⟩ ---> *)
-  (*   ⟨ δ , stm_if e (stm_seq s (stm_while w e s)) (stm_lit tt) ⟩ *)
-  | step_stm_match_list
-      (δ : LocalStore Γ) {σ τ : Ty} (e : Exp Γ (ty_list σ)) (alt_nil : Stm Γ τ)
-      (xh xt : 𝑿) (alt_cons : Stm (Γ ▻ (xh , σ) ▻ (xt , ty_list σ)) τ) :
-      ⟨ δ , stm_match_list e alt_nil xh xt alt_cons ⟩ --->
-      ⟨ δ , match eval e δ with
-            | nil => alt_nil
-            | cons vh vt => stm_let' (env_snoc (env_snoc env_nil (xh,σ) vh) (xt,ty_list σ) vt) alt_cons
-            end
-      ⟩
-  | step_stm_match_sum
-      (δ : LocalStore Γ) {σinl σinr τ : Ty} (e : Exp Γ (ty_sum σinl σinr))
-      (xinl : 𝑿) (alt_inl : Stm (Γ ▻ (xinl , σinl)) τ)
-      (xinr : 𝑿) (alt_inr : Stm (Γ ▻ (xinr , σinr)) τ) :
-      ⟨ δ , stm_match_sum e xinl alt_inl xinr alt_inr ⟩ --->
-      ⟨ δ , match eval e δ with
-            | inl v => stm_let' (env_snoc env_nil (xinl,σinl) v) alt_inl
-            | inr v => stm_let' (env_snoc env_nil (xinr,σinr) v) alt_inr
-            end
-      ⟩
-  | step_stm_match_pair
-      (δ : LocalStore Γ) {σ1 σ2 τ : Ty} (e : Exp Γ (ty_prod σ1 σ2)) (xl xr : 𝑿)
-      (rhs : Stm (Γ ▻ (xl , σ1) ▻ (xr , σ2)) τ) :
-      ⟨ δ , stm_match_pair e xl xr rhs ⟩ --->
-      ⟨ δ , let (vl , vr) := eval e δ in
-            stm_let' (env_snoc (env_snoc env_nil (xl,σ1) vl) (xr,σ2) vr) rhs
-      ⟩
-  | step_stm_match_enum
-      (δ : LocalStore Γ) {E : 𝑬} (e : Exp Γ (ty_enum E)) {τ : Ty}
-      (alts : forall (K : 𝑬𝑲 E), Stm Γ τ) :
-      ⟨ δ , stm_match_enum E e alts ⟩ ---> ⟨ δ , alts (eval e δ) ⟩
-  | step_stm_match_tuple
-      (δ : LocalStore Γ) {σs : Ctx Ty} {Δ : Ctx (𝑿 * Ty)}
-      (e : Exp Γ (ty_tuple σs)) (p : TuplePat σs Δ)
-      {τ : Ty} (rhs : Stm (ctx_cat Γ Δ) τ) :
-      ⟨ δ , stm_match_tuple e p rhs ⟩ --->
-      ⟨ δ , stm_let' (tuple_pattern_match p (eval e δ)) rhs ⟩
-
-  | step_stm_match_union
-      (δ : LocalStore Γ) {T : 𝑻} (e : Exp Γ (ty_union T)) {τ : Ty}
-      (altx : forall (K : 𝑲 T), 𝑿)
-      (alts : forall (K : 𝑲 T), Stm (ctx_snoc Γ (altx K , 𝑲_Ty K)) τ) :
-      ⟨ δ , stm_match_union T e altx alts ⟩ --->
-      ⟨ δ , let (K , v) := eval e δ in
-            stm_let' (env_snoc env_nil (altx K,𝑲_Ty K) (untag v)) (alts K)
-      ⟩
-  | step_stm_match_record
-      (δ : LocalStore Γ) {R : 𝑹} {Δ : Ctx (𝑿 * Ty)}
-      (e : Exp Γ (ty_record R)) (p : RecordPat (𝑹𝑭_Ty R) Δ)
-      {τ : Ty} (rhs : Stm (ctx_cat Γ Δ) τ) :
-      ⟨ δ , stm_match_record R e p rhs ⟩ --->
-      ⟨ δ , stm_let' (record_pattern_match p (eval e δ)) rhs ⟩
+      (e1 : bool) (e2 : string) :
+      stm_assert e1 e2 --->
+      if e1 then stm_lit true else stm_exit bool e2
 
   | step_stm_bind_step
-      (δ δ' : LocalStore Γ) (σ τ : Ty) (s s' : Stm Γ σ) (k : Lit σ -> Stm Γ τ) :
-      ⟨ δ , s ⟩ ---> ⟨ δ' , s' ⟩ ->
-      ⟨ δ , stm_bind s k ⟩ ---> ⟨ δ' , stm_bind s' k ⟩
+      (σ τ : Set) `{Blastable σ} (s s' : Stm σ) (k : σ -> Stm τ) :
+      s ---> s' ->
+      stm_bind s k ---> stm_bind s' k
   | step_stm_bind_value
-      (δ : LocalStore Γ) (σ τ : Ty) (v : Lit σ) (k : Lit σ -> Stm Γ τ) :
-      ⟨ δ , stm_bind (stm_lit σ v) k ⟩ ---> ⟨ δ , k v ⟩
+      (σ τ : Set) `{Blastable σ} (v : σ) (k : σ -> Stm τ) :
+      stm_bind (stm_lit v) k ---> k v
   | step_stm_bind_exit
-      (δ : LocalStore Γ) (σ τ : Ty) (s : string) (k : Lit σ -> Stm Γ τ) :
-      ⟨ δ , stm_bind (stm_exit σ s) k ⟩ ---> ⟨ δ , stm_exit τ s ⟩
+      (σ τ : Set)  `{Blastable σ} (s : string) (k : σ -> Stm τ) :
+      stm_bind (stm_exit σ s) k ---> stm_exit τ s
+  where "s1 '--->' s2" := (Step s1 s2).
 
-  where "'⟨' δ1 ',' s1 '⟩' '--->' '⟨' δ2 ',' s2 '⟩'" := (@Step _ _ δ1 δ2 s1 s2).
+  Inductive Steps {σ : Set} (s1 : Stm σ) : Stm σ -> Prop :=
+  | step_refl : Steps s1 s1
+  | step_trans {s2 s3 : Stm σ} :
+      Step s1 s2 -> Steps s2 s3 -> Steps s1 s3.
 
-  Inductive Steps {Γ : Ctx (𝑿 * Ty)} {σ : Ty} (δ1 : LocalStore Γ) (s1 : Stm Γ σ) : LocalStore Γ -> Stm Γ σ -> Prop :=
-  | step_refl : Steps δ1 s1 δ1 s1
-  | step_trans {δ2 δ3 : LocalStore Γ} {s2 s3 : Stm Γ σ} :
-      Step δ1 δ2 s1 s2 -> Steps δ2 s2 δ3 s3 -> Steps δ1 s1 δ3 s3.
+  Notation "s1 ---> s2" := (Step s1 s2).
+  Notation "s1 --->* s2" := (Steps s1 s2).
 
-  Notation "'⟨' δ1 ',' s1 '⟩' '--->' '⟨' δ2 ',' s2 '⟩'" := (@Step _ _ δ1 δ2 s1 s2).
-  Notation "'⟨' δ1 ',' s1 '⟩' --->* '⟨' δ2 ',' s2 '⟩'" := (@Steps _ _ δ1 s1 δ2 s2).
+  (* Definition Triple {Γ τ} *)
+  (*   (PRE : Pred (LocalStore Γ)) (s : Stm τ) *)
+  (*   (POST : Lit τ -> Pred (LocalStore Γ)) : Prop := *)
+  (*   forall (δ δ' : LocalStore Γ) (v : Lit τ), *)
+  (*     ⟨ δ , s ⟩ --->* ⟨ δ' , stm_lit τ v ⟩ -> *)
+  (*     PRE δ -> *)
+  (*     POST v δ'. *)
+
+  (* Definition TripleNoExit {Γ τ} *)
+  (*   (PRE : Pred (LocalStore Γ)) (s : Stm τ) *)
+  (*   (POST : Lit τ -> Pred (LocalStore Γ)) : Prop := *)
+  (*   forall (δ δ' : LocalStore Γ) (s' : Stm τ), *)
+  (*     ⟨ δ, s ⟩ --->* ⟨ δ', s' ⟩ -> *)
+  (*     Final s' -> *)
+  (*     PRE δ -> *)
+  (*     IsLit δ' s' POST. *)
 
 End SmallStep.
